Factor out common tactics and lemmas from X64 and AArch64.

Kraken/AArch64/Semantics.lean
@@ -1,8 +1,8 @@
+import Kraken.AArch64.Syntax
+import Kraken.Attribute
+import Kraken.Mem
 import Lean
 import Std
-import Kraken.AArch64.Syntax
-import Kraken.Mem
-import Kraken.Attribute
 
 -- injective coercions only
 attribute [-instance] BitVec.instNatCast
@@ -949,33 +949,12 @@ def Directives.interp [Labels]
     d.interp s (.mk pc (pc+.ofNat sz)) (jmp:=ret) (next := (fun s =>
     interp ds s (pc+.ofNat sz) ret))
 
-class Layout where (start : Int64) (size : Nat → Nat)
-def Layout.apply (l : Layout) (prog : Program) : Executable :=
-  (l.start, prog.mapIdx (fun i d => (d, l.size i)))
-instance : CoeFun Layout (fun _ => Program → Executable) where coe := Layout.apply
-
--- Returns each directive paired with its start address and size.
--- TODO: tail-recursive version for efficiency?
-def Executable.withAddresses (e : Executable): List (Int64 × Directive × Nat) :=
-  let (start_addr, ds) := e
-  match ds with
-  | [] => []
-  | (instr, instr_sz) :: ds =>
-    (start_addr, instr, instr_sz) :: Executable.withAddresses (start_addr + .ofNat instr_sz, ds)
-termination_by e.2
+abbrev Layout := Kraken.Layout Directive
 
 @[reducible]
 def Executable.labels (e : Executable) : Labels :=
   { label l := (e.withAddresses.findSome?
       (fun (p, d, _) => if d = .label l then .some p else .none)).getD (-1) }
-
-def Executable.directivesAtAddress (e : Executable) (a : Int64) : List (Directive × Nat) :=
-  let starts_at_a := e.withAddresses.dropWhile (·.1 ≠ a)
-  (starts_at_a.takeWhile (·.1 = a)).map (·.2)
-
-def Executable.directivesFromAddress (e : Executable) (a : Int64) : List (Directive × Nat) :=
-  let starts_at_a := e.withAddresses.dropWhile (·.1 ≠ a)
-  starts_at_a.map (·.2)
 
 def Executable.directivesFromLabel (e : Executable) (l : Label) : List (Directive × Nat) :=
   e.2.dropWhile (·.1 != .label l)
@@ -983,17 +962,17 @@ def Executable.directivesFromLabel (e : Executable) (l : Label) : List (Directiv
 abbrev MachineState := MachineData × Int64
 
 def Executable.step (e : Executable) (s : MachineState) (ret : MachineState → Effects) : Effects :=
-  let := e.labels
+  let := Executable.labels e
   Directives.interp (e.directivesAtAddress s.2) s.1 s.2 (fun pc s => ret (s, pc))
 
 def Executable.straightline (e : Executable) (s : MachineState) (ret : MachineState → Effects) : Effects :=
-  let := e.labels;
+  let := Executable.labels e
   Directives.interp (e.directivesFromAddress s.2) s.1 s.2 (fun pc s => ret (s, pc))
 
 -- -- Concrete evaluators for expedient testing
 
 partial def Executable.eval (e : Executable) (s : MachineState) (until_ : MachineState → Bool) : Except String (MachineState) :=
-  if until_ s then .ok s else handleEffects (e.straightline s .done)
+  if until_ s then .ok s else handleEffects (Executable.straightline e s .done)
 where
   handleEffects es :=
     match es with
@@ -1019,7 +998,7 @@ def Program.fakeLayout (prog : Program) : Executable :=
   let layout : Layout := { start := h.toInt64<<<16, size i := prog[i]!.fakeSize }
   layout prog
 
-abbrev eval [layout : Layout] (prog : Program) := (layout prog).eval
+abbrev eval [layout : Layout] (prog : Program) := Executable.eval (layout prog)
 
 /-- info: Except.ok 58 -/
 #guard_msgs in
@@ -1030,9 +1009,9 @@ abbrev eval [layout : Layout] (prog : Program) := (layout prog).eval
     .instr ⟨.W64, .ADD_e .X1 .X1 0x10⟩,
     .instr ⟨.W64, .STR .X1 { base := .SP, off := 0 }⟩,
     .instr ⟨.W64, .LDR .X2 (.addr { base := .SP, off := 0 })⟩]
-  let start := exe.labels.label "main"
-  let data := { dmem := Mem.storeInt {} 0x100 8 42, regs := {SP := 0x100} }
-  (exe.eval (data, start) (fun (_, pc) => (exe.directivesFromAddress pc).isEmpty)).bind (fun s => .ok s.1.regs.X2)
+  let start := (Executable.labels exe).label "main"
+  let data : MachineData := { dmem := Mem.storeInt {} 0x100 8 42, regs := {SP := 0x100} }
+  (Executable.eval exe (data, start) (fun (_, pc) => (exe.directivesFromAddress pc).isEmpty)).bind (fun s => .ok s.1.regs.X2)
 
 /-- info: Except.ok (42, 264) -/
 #guard_msgs in
@@ -1040,9 +1019,9 @@ abbrev eval [layout : Layout] (prog : Program) := (layout prog).eval
   let exe := Program.fakeLayout [
     .label "main",
     .instr ⟨.W64, .LDR .X1 (.addr { base := .SP, off := .imm { imm := 8, index := some .Pre } })⟩ ]
-  let start := exe.labels.label "main"
-  let data := { dmem := Mem.storeInt {} 0x108 8 42, regs := { SP := 0x100 } }
-  (exe.eval (data, start) (fun (_, pc) => (exe.directivesFromAddress pc).isEmpty)).bind (fun s => .ok (s.1.regs.X1, s.1.regs.SP))
+  let start := (Executable.labels exe).label "main"
+  let data : MachineData := { dmem := Mem.storeInt {} 0x108 8 42, regs := { SP := 0x100 } }
+  (Executable.eval exe (data, start) (fun (_, pc) => (exe.directivesFromAddress pc).isEmpty)).bind (fun s => .ok (s.1.regs.X1, s.1.regs.SP))
 
 /-- info: Except.ok (42, 264) -/
 #guard_msgs in
@@ -1050,9 +1029,9 @@ abbrev eval [layout : Layout] (prog : Program) := (layout prog).eval
   let exe := Program.fakeLayout [
     .label "main",
     .instr ⟨.W64, .STR .X1 { base := .SP, off := .imm { imm := 8, index := some .Post } }⟩ ]
-  let start := exe.labels.label "main"
-  let data := { dmem := Mem.storeInt {} 0x100 8 0, regs := { SP := 0x100, X1 := 42 } }
-  (exe.eval (data, start) (fun (_, pc) => (exe.directivesFromAddress pc).isEmpty)).bind (fun s =>
+  let start := (Executable.labels exe).label "main"
+  let data : MachineData := { dmem := Mem.storeInt {} 0x100 8 0, regs := { SP := 0x100, X1 := 42 } }
+  (Executable.eval exe (data, start) (fun (_, pc) => (exe.directivesFromAddress pc).isEmpty)).bind (fun s =>
     match Mem.loadInt s.1.dmem 0x100 8 with
     | some v => .ok (v, s.1.regs.SP)
     | none => .error "Memory store failed"
