KrakenAArch64.lean
@@ -4,11 +4,9 @@
   Root module that re-exports all AArch64 Kraken components.
 -/
 
-import Kraken.AArch64.Semantics
-import Kraken.AArch64.OmniSemantics
-import Kraken.AArch64.Sep
-import Kraken.AArch64.Tactics
-import Kraken.AArch64.Parser
-import Kraken.AArch64.Tactics
-import Kraken.AArch64.Sep
 import Kraken.AArch64.Examples.Examples
+import Kraken.AArch64.OmniSemantics
+import Kraken.AArch64.Parser
+import Kraken.AArch64.Semantics
+import Kraken.AArch64.Sep
+import Kraken.Tactics
