KrakenRunnerAArch64.lean
@@ -11,8 +11,8 @@ Output:
 - Json formatted Machine state of Kraken after running the assembly.
 -/
 
-import Kraken.AArch64.Semantics
 import Kraken.AArch64.Parser
+import Kraken.AArch64.Semantics
 import Kraken.Mem
 import Lean.Data.Json
 
